imp/Imp2ClightSim.v
@@ -1,0 +1,139 @@
+From compcert Require Import Smallstep Clight Integers Events Behaviors.
+Require Import Coqlib.
+Require Import Universe.
+Require Import STS.
+Require Import Behavior.
+Require Import Imp.
+Require Import Imp2Clight.
+
+Set Implicit Arguments.
+
+Definition single_events_at (L: Smallstep.semantics) (s:L.(Smallstep.state)) : Prop :=
+  forall t s', Step L s t s' -> (t = E0).
+
+Record strict_determinate_at (L: Smallstep.semantics) (s:L.(Smallstep.state)) : Prop :=
+  Strict_determinate_at {
+      ssd_determ_at: forall t1 s1 t2 s2
+        (STEP0: Step L s t1 s1)
+        (STEP1 :Step L s t2 s2),
+        <<EQ: s1 = s2>>;
+    ssd_determ_at_final: forall tr s' retv
+        (FINAL: Smallstep.final_state L s retv)
+        (STEP: Step L s tr s'),
+        False;
+    ssd_traces_at:
+      single_events_at L s
+  }.
+
+Section SIM.
+
+  Variable L0: STS.semantics.
+  Variable L1: Smallstep.semantics.
+  Variable idx: Type.
+  Variable ord: idx -> idx -> Prop.
+
+  Local Open Scope smallstep_scope.
+
+  Variant _sim sim (i0: idx) (st_src0: L0.(STS.state)) (st_tgt0: L1.(Smallstep.state)): Prop :=
+  | sim_fin
+      retv
+      (RANGE: (0 <= retv <= Int.max_unsigned)%Z)
+      (SRT: _.(state_sort) st_src0 = final retv)
+      (SRT: _.(Smallstep.final_state) st_tgt0 (Int.repr retv))
+      (DTM: True) (*** TODO: copy-paste sd_final_determ in Smallstep.v ***)
+    :
+      _sim sim i0 st_src0 st_tgt0
+
+  (* | sim_vis *)
+  (*     (SRT: _.(state_sort) st_src0 = vis) *)
+  (*     (SRT: _.(state_sort) st_tgt0 = vis) *)
+  (*     (SIM: forall ev st_tgt1 *)
+  (*         (STEP: _.(step) st_tgt0 (Some ev) st_tgt1) *)
+  (*       , *)
+  (*         exists st_src1 (STEP: _.(step) st_src0 (Some ev) st_src1), *)
+  (*           <<SIM: exists i1, sim i1 st_src1 st_tgt1>>) *)
+  (*   : *)
+  (*     _sim sim i0 st_src0 st_tgt0 *)
+
+  | sim_demonic_src
+      (SRT: _.(state_sort) st_src0 = demonic)
+      (SIM: exists st_src1
+          (STEP: _.(step) st_src0 None st_src1)
+        ,
+          exists i1, <<ORD: ord i1 i0>> /\ <<SIM: sim i1 st_src1 st_tgt0>>)
+    :
+      _sim sim i0 st_src0 st_tgt0
+  | sim_demonic_tgt_dtm
+      (*** WRONG DEF, Note: UB in tgt ***)
+      (* (SIM: forall st_tgt1 *)
+      (*     (STEP: Step L1 st_tgt0 E0 st_tgt1) *)
+      (*   , *)
+      (*     exists i1, <<ORD: ord i1 i0>> /\ <<SIM: sim i1 st_src0 st_tgt1>>) *)
+      (DTM: strict_determinate_at L1 st_tgt0)
+      (SIM: exists st_tgt1
+          (STEP: Step L1 st_tgt0 E0 st_tgt1)
+        ,
+          exists i1, <<ORD: ord i1 i0>> /\ <<SIM: sim i1 st_src0 st_tgt1>>)
+      (*** equivalent def ***)
+      (* st_tgt1 *)
+      (* (STEP: Step L1 st_tgt0 E0 st_tgt1) *)
+      (* i1 *)
+      (* (ORD: ord i1 i0) *)
+      (* (SIM: sim i1 st_src0 st_tgt1) *)
+    :
+      _sim sim i0 st_src0 st_tgt0
+  | sim_angelic_src
+      (SRT: _.(state_sort) st_src0 = angelic)
+      (SIM: forall st_src1
+          (STEP: _.(step) st_src0 None st_src1)
+        ,
+          exists i1, <<ORD: ord i1 i0>> /\ <<SIM: sim i1 st_src1 st_tgt0>>)
+    :
+      _sim sim i0 st_src0 st_tgt0
+
+
+  | sim_demonic_both
+      (SRT: _.(state_sort) st_src0 = demonic)
+      (DTM: strict_determinate_at L1 st_tgt0)
+      (SIM: exists st_tgt1
+          (STEP: Step L1 st_tgt0 E0 st_tgt1)
+        ,
+          exists st_src1 (STEP: _.(step) st_src0 None st_src1),
+            <<SIM: exists i1, sim i1 st_src1 st_tgt1>>)
+    :
+      _sim sim i0 st_src0 st_tgt0
+  .
+
+  Definition sim: _ -> _ -> _ -> Prop := paco3 _sim bot3.
+
+  Lemma sim_mon: monotone3 _sim.
+  Proof.
+    ii. inv IN.
+
+    - econs 1; et.
+    - econs 2; et. des. esplits; et.
+    - econs 3; et. des. esplits; et.
+    - econs 4; et. i. exploit SIM; et. i; des. esplits; et.
+    - econs 5; et. des. esplits; et.
+  Qed.
+
+  Hint Constructors _sim.
+  Hint Unfold sim.
+  Hint Resolve sim_mon: paco.
+
+  Record simulation: Prop := mk_simulation {
+    sim_wf_ord: <<WF: well_founded ord>>;
+    sim_init: forall st_tgt0 (INITT: L1.(Smallstep.initial_state) st_tgt0),
+        exists i0, (<<SIM: sim i0 L0.(initial_state) st_tgt0>>);
+    (* sim_init: exists i0 st_tgt0, (<<SIM: sim i0 L0.(initial_state) st_tgt0>>) /\ *)
+    (*                              (<<INITT: L1.(Smallstep.initial_state) st_tgt0>>); *)
+    (* sim_dtm: True; *)
+  }
+  .
+
+  Hypothesis WF: well_founded ord.
+
+  Ltac pc H := rr in H; desH H; ss.
+
+End SIM.
+
